Removing old definitions from CoherenceTop.

withtop/Proofs/CoherenceTop.v
@@ -73,20 +73,25 @@ Inductive Atomic : PTyp -> Prop :=
   | AInt : Atomic PInt
   | AFun : forall t1 t2, Atomic (Fun t1 t2).
 
-Fixpoint genCoerce (n : nat) : Exp :=
-  match n with
-    | 0 => fun A => STLam' _ (STUnit _)
-    | S m => fun A => STLam' _ (genCoerce m A)
+Inductive TopSig : PTyp -> Prop :=
+  | TopSigF : forall A B, TopSig B -> TopSig (Fun A B)
+  | TopSigT : TopSig TopT.  
+
+Fixpoint and_coercion (t : PTyp) (e : Exp) {struct t} : sum Exp Exp :=
+  match t with
+    | PInt    => inr e
+    | Fun _ B => match (and_coercion B e) with
+                  | inl l => inl (fun A : Type => STLam' A (l A))
+                  | inr r => inr r
+                 end 
+    | And _ _ => inr e
+    | TopT    => inl (fun A => (STUnit A))
   end.
 
-Fixpoint and_coercion (t : PTyp) (e1 : Exp) (n : nat) : Exp :=
-  match t with
-    | PInt => e1
-    | TopT => genCoerce n
-    | Fun A B => and_coercion B e1 (S n)
-    | And A B => e1
-  end.
-  
+Definition join_sum : forall {A}, A + A -> A.
+  intros A H; destruct H as [a | a]; exact a.
+Defined.
+
 Inductive sub : PTyp -> PTyp -> Exp -> Prop :=
   | SInt : sub PInt PInt (fun A => STLam' _ (STBVar _ 0))
   | SFun : forall o1 o2 o3 o4 c1 c2, sub o3 o1 c1 -> sub o2 o4 c2 -> 
@@ -96,12 +101,83 @@ Inductive sub : PTyp -> PTyp -> Exp -> Prop :=
      sub t (And  t1 t2) (fun A => STLam' _ (
        STPair _ (STApp _ (c1 A) (STBVar _ 0)) (STApp _ (c2 A) (STBVar _ 0))))
   | SAnd2 : forall t t1 t2 c, sub t1 t c -> Atomic t ->
-     sub (And  t1 t2) t (and_coercion t (fun A => STLam' _ (
-       (STApp _ (c A) (STProj1 _ (STBVar _ 0))))) 0)
+     sub (And  t1 t2) t (fun A => STLam' _ (join_sum (and_coercion t (fun A => (
+       (STApp _ (c A) (STProj1 _ (STBVar _ 0)))))) A))
   | SAnd3 : forall t t1 t2 c, sub t2 t c -> Atomic t ->
-     sub (And  t1 t2) t (and_coercion t (fun A => STLam' _ (
-       (STApp _ (c A) (STProj2 _ (STBVar _ 0))))) 0)
+     sub (And  t1 t2) t (fun A => STLam' _ (join_sum (and_coercion t (fun A => (
+       (STApp _ (c A) (STProj2 _ (STBVar _ 0)))))) A))
   | STop : forall t, sub t TopT (fun A => STLam' _ (STUnit _)).
+
+Notation "'|' t '|'" := (ptyp2styp t) (at level 60).
+
+Lemma and_coercion_inl_term :
+  forall {t e},
+    TopSig t ->
+    exists r, and_coercion t e = inl r /\ STTerm (r var).  
+Proof.
+  intros.
+  induction H.
+  inversion IHTopSig.
+  exists (fun A : Type => STLam' A (x A)).
+  inversion H0.
+  split.
+  simpl.
+  rewrite H1.
+  reflexivity.
+  apply_fresh STTerm_Lam' as x.
+  unfold open; rewrite <- open_rec_term; auto.
+  exists (fun A : Type => STUnit A); auto.
+Qed.
+  
+Lemma and_coercion_inl_typing :
+  forall {t e Gamma},
+    ok Gamma ->
+    TopSig t ->
+    exists r, and_coercion t e = inl r /\ has_type_st Gamma (r var) (|t|).  
+Proof.
+  intros.
+  induction H0.
+  destruct IHTopSig.
+  exists (fun A : Type => STLam' A (x A)).
+  simpl.
+  destruct H1.
+  rewrite H1.
+  split.
+  reflexivity.
+  apply_fresh STTyLam' as v.
+  unfold open.
+  rewrite <- open_rec_term.
+  rewrite <- app_nil_l with (l := extend v (| A |) Gamma).
+  apply typing_weaken; rewrite app_nil_l.
+  apply H2.
+  apply Ok_push; assumption.
+  now apply typing_gives_terms in H2.
+  exists (fun A : Type =>  STUnit A).
+  split.
+  now simpl.
+  simpl.
+  apply STTyUnit.
+  auto.
+Qed.
+
+Lemma and_coercion_inr :
+  forall {t e},
+    not (TopSig t) ->
+    and_coercion t e = inr e.
+Proof.
+  intros.
+  generalize dependent e.
+  induction t0; try simpl; auto.
+  intros.
+  assert (not (TopSig t0_2)).
+  unfold not; intros HTS; apply H.
+  apply TopSigF; apply HTS.
+  apply IHt0_2 with (e := e) in H0.
+  rewrite H0.
+  reflexivity.
+  exfalso; apply H; apply TopSigT.
+Qed.
+
 
 Definition Sub (t1 t2 : PTyp) : Prop := exists (e:Exp), sub t1 t2 e.
 
@@ -134,11 +210,11 @@ Defined.
 
 Definition sand2_atomic : forall t t1 t2, Sub t1 t -> Atomic t -> Sub (And  t1 t2) t.
 unfold Sub. intro t. intros. destruct t. destruct H.
-exists (and_coercion PInt (fun A => STLam' _ (
-       (STApp _ (x A) (STProj1 _ (STBVar _ 0))))) 0).
+exists (fun A => STLam' _ (join_sum (and_coercion PInt (fun A => (
+       (STApp _ (x A) (STProj1 _ (STBVar _ 0)))))) A)).
 apply SAnd2. auto. auto. destruct H.
-exists (and_coercion (Fun t3 t4) (fun A => STLam' _ ( 
-       (STApp _ (x A) (STProj1 _ (STBVar _ 0))))) 0).
+exists (fun A => STLam' _ (join_sum (and_coercion (Fun t3 t4) (fun A => (
+       (STApp _ (x A) (STProj1 _ (STBVar _ 0)))))) A)).
 apply SAnd2. auto. auto.
 inversion H0.
 apply stop. (* a top case here *)
@@ -172,12 +248,12 @@ apply stop. (* a top case here *)
 Defined.
 
 Definition sand3_atomic : forall t t1 t2, Sub t2 t -> Atomic t -> Sub (And  t1 t2) t.
-unfold Sub. intro t; intros. destruct t. destruct H.
-exists (and_coercion PInt (fun A => STLam' _ ( 
-       (STApp _ (x A) (STProj2 _ (STBVar _ 0))))) 0).
+  unfold Sub. intro t; intros. destruct t. destruct H.
+  exists (fun A => STLam' _ (join_sum (and_coercion PInt (fun A => (
+       (STApp _ (x A) (STProj2 _ (STBVar _ 0)))))) A)).
 apply SAnd3. auto. auto. destruct H.
-exists (and_coercion (Fun t3 t4) (fun A => STLam' _ ( 
-       (STApp _ (x A) (STProj2 _ (STBVar _ 0))))) 0).
+exists (fun A => STLam' _ (join_sum (and_coercion (Fun t3 t4) (fun A => (
+       (STApp _ (x A) (STProj2 _ (STBVar _ 0)))))) A)).
 apply SAnd3. auto. auto.
 inversion H0.
 apply stop. (* a top case here *)
@@ -492,7 +568,8 @@ unfold Sub. exists c2. auto.
 apply TLTop.
 Defined.
 
-Lemma same_coercion : forall B, TopLike B -> WFTyp B -> forall A e1 e2 n, and_coercion (Fun A B) e1 n = and_coercion (Fun A B) e2 n.
+Lemma same_coercion : forall B, TopLike B -> WFTyp B -> forall A e1 e2,
+  and_coercion (Fun A B) e1 = and_coercion (Fun A B) e2.
 intro. intro.
 induction H; intros.
 (* Case TopT *)
@@ -504,7 +581,7 @@ simpl. inversion H1. destruct H6. destruct H6. contradiction.
 (* Case Fun *)
 simpl in IHTopLike.
 simpl. inversion H0.
-apply IHTopLike. auto. apply A0.
+rewrite IHTopLike with (e2 := e2); auto.
 Defined.
 
 (* Coercive subtyping is coeherent: Lemma 5 *)
@@ -545,7 +622,8 @@ assert (TopLike t0). apply H15. unfold Sub.
 exists c; auto. unfold Sub. exists c0. auto.
 inversion H16. rewrite <- H17 in H2. inversion H2.
 rewrite <- H19 in H2. inversion H2.
-apply same_coercion. auto. rewrite <- H18 in H0. inversion H0. auto.
+erewrite same_coercion; auto.
+rewrite <- H18 in H0. inversion H0. auto.
 (* top case *)
 rewrite <- H5 in H2. inversion H2.
 (* Case: And t1 t2 <: t (second) *)
@@ -559,7 +637,7 @@ unfold Sub. exists c0. auto.
 unfold Sub. exists c. auto.
 inversion H18. rewrite <- H19 in H2. inversion H2.
 rewrite <- H21 in H2. inversion H2.
-apply same_coercion. auto. rewrite <- H20 in H0. inversion H0. auto.
+erewrite same_coercion; auto. rewrite <- H20 in H0. inversion H0. auto.
 (* same coercion; no contradiction *)
 assert (c = c0). apply IHsub; auto. rewrite H15.
 reflexivity.
@@ -695,7 +773,6 @@ Definition open_source t u := open_rec_source 0 u t.
 Definition conv_context (env : context PTyp) : context STyp :=
   mapctx ptyp2styp env.
 
-Notation "'|' t '|'" := (ptyp2styp t) (at level 60).
 Notation "'∥' t '∥'" := (conv_context t) (at level 60).
 
 Lemma ok_map : forall Gamma, ok Gamma -> ok (∥ Gamma ∥).
@@ -1606,8 +1683,6 @@ Definition body_typ t A B Gamma E :=
   exists L, forall x, not (In x L) -> has_type_source_alg (extend x A Gamma) (open_source t (PFVar x)) Chk B (open E (STFVar _ x)).
 
 (** We then show how to introduce and eliminate [body t]. *)
-Print has_type_source_alg.
-
 Lemma term_abs_to_body_typ : forall t1 A B Gamma E, 
   has_type_source_alg Gamma (PLam t1) Chk (Fun A B) (STLam' _ E) -> body_typ t1 A B Gamma E.
 Proof. intros. unfold body_typ. inversion H. subst. exists L. unfold open_rec. apply H5. Qed.
@@ -1979,8 +2054,6 @@ Proof.
   right; apply IHGamma; auto.
 Defined.
 
-Print open_rec_source.
-
 Lemma open_rec_term_core :
   forall t j v i u, i <> j -> open_rec_source j (PFVar v) t = open_rec_source i (PFVar u) (open_rec_source j (PFVar v) t) ->
     t = open_rec_source i (PFVar u) t.
@@ -2029,59 +2102,219 @@ Proof.
   - reflexivity.
 Defined.
 
-Lemma and_coercion_proj1_term :
-  forall t0 n (c : Exp),
-    STTerm (c var) ->
-    STTerm (and_coercion t0 (fun A : Type =>
-                               STLam' A (STApp A (c A) (STProj1 A
-                                                                (STBVar A 0)))) n
-        var).
+Lemma topsig_dec : forall t, sumbool (TopSig t) (not (TopSig t)).
+Proof.
+  intro t.
+  induction t.
+  - right; unfold not; intros HInv; inversion HInv. 
+  - inversion IHt2.
+    left.
+    apply TopSigF.
+    apply H.
+    right.
+    unfold not; intros HInv; inversion HInv; subst.
+    contradiction.
+  - right; unfold not; intros HInv; inversion HInv.
+  - left; apply TopSigT.
+Qed.    
+
+(* Subtyping rules produce type-correct coercions: Lemma 3 *)
+Lemma type_correct_coercions :
+  forall Gamma A B E, sub A B E ->
+             ok Gamma -> 
+             has_type_st Gamma (E var) (STFun (|A|) (|B|)) .
 Proof.
   intros.
-  generalize dependent n.
-  induction t0; intros; simpl; try apply IHt0_2.
-  - apply_fresh STTerm_Lam' as x; cbn.
-    apply STTerm_App; auto.
-    rewrite <- open_rec_term; auto.
-  - apply_fresh STTerm_Lam' as x; cbn.
-    apply STTerm_App; auto.
-    rewrite <- open_rec_term; auto.
-  - induction n.
+  induction H.
+  (* Case SInt *)
+  - simpl.
+    apply_fresh STTyLam' as x; cbn.
+    simpl; apply STTyVar.
+    apply Ok_push; auto.
+    left; simpl; auto.
+  (* Case SFun *)
+  - apply_fresh STTyLam' as x; cbn.
+    apply_fresh STTyLam' as y; cbn.
+    apply STTyApp with (A := (| o2 |)).
+    rewrite <- open_rec_term.
+    rewrite <- open_rec_term.
+    repeat apply typing_weaken_extend.
+    assumption.
+    assumption. 
     simpl.
-    apply_fresh STTerm_Lam' as x; auto.
+    not_in_L y.
+    apply MSetProperties.Dec.F.add_iff in H4; inversion H4.
+    exfalso; apply H2; apply MSetProperties.Dec.F.singleton_2; auto.
+    assumption.
+    now apply typing_gives_terms in IHsub2.
+    rewrite <- open_rec_term.
+    now apply typing_gives_terms in IHsub2.
+    now apply typing_gives_terms in IHsub2.
+    eapply STTyApp.
+    apply STTyVar.
+    apply Ok_push.
+    apply Ok_push.
+    assumption.
+    assumption.
+    not_in_L y.
+    not_in_L x.
+    right; left; reflexivity.
+    apply STTyApp with (A := (| o3 |)).
+    rewrite <- open_rec_term.
+    rewrite <- open_rec_term.
+    repeat apply typing_weaken_extend.
+    assumption.
+    assumption. 
     simpl.
-    apply_fresh STTerm_Lam' as x; simpl in *.
-    unfold open.
-    rewrite <- open_rec_term; auto.
+    not_in_L y.
+    apply MSetProperties.Dec.F.add_iff in H4; inversion H4.
+    exfalso; apply H2; apply MSetProperties.Dec.F.singleton_2; auto.
+    assumption.
+    now apply typing_gives_terms in IHsub1.
+    rewrite <- open_rec_term; now apply typing_gives_terms in IHsub1.
+    apply STTyVar.
+    apply Ok_push.
+    apply Ok_push.
+    assumption.
+    assumption.
+    simpl.
+    rewrite union_spec in Fry.
+    apply not_or_and in Fry.
+    inversion Fry.
+    unfold not; intros.
+    apply MSetProperties.Dec.F.add_iff in H4.
+    inversion H4.
+    apply H2.
+    apply MSetProperties.Dec.F.singleton_2; assumption.
+    contradiction.
+    left; reflexivity.
+  (* Case SAnd1 *)
+  - apply_fresh STTyLam' as x; cbn.
+    apply STTyPair.
+    eapply STTyApp.
+    rewrite <- open_rec_term.
+    apply typing_weaken_extend.
+    apply IHsub1.
+    assumption.
+    now apply typing_gives_terms in IHsub1.
+    apply STTyVar.
+    apply Ok_push; auto.
+    left; reflexivity.
+    eapply STTyApp.
+    rewrite <- open_rec_term.
+    apply typing_weaken_extend.
+    apply IHsub2.
+    assumption.
+    now apply typing_gives_terms in IHsub2.
+    apply STTyVar.
+    apply Ok_push; auto.
+    left; reflexivity.
+  - pose (topsig_dec t0).
+    inversion s; clear s.
+    assert (Ha : exists r, and_coercion t0 ((fun A : Type => STApp A (c A) (STProj1 A (STBVar A 0)))) = inl r /\ has_type_st Gamma (r var) (|t0|)) by (apply and_coercion_inl_typing; auto).
+    destruct Ha as [r [HCoerce HHasTy]].
+    rewrite HCoerce.
+    apply_fresh STTyLam' as x.
+    simpl.
+    unfold open; rewrite <- open_rec_term.
+    rewrite <- app_nil_l with (l := (extend x (STTuple (| t1 |) (| t2 |)) Gamma)).
+    apply typing_weaken; rewrite app_nil_l.
+    apply HHasTy.
+    apply Ok_push; auto.
+    now apply typing_gives_terms in HHasTy.
+    eapply and_coercion_inr in H2.
+    rewrite H2; simpl.
+    apply_fresh STTyLam' as x; cbn.
+    eapply STTyApp.
+    rewrite <- open_rec_term.
+    apply typing_weaken_extend.
+    apply IHsub.
+    assumption.
+    now apply typing_gives_terms in IHsub.
+    eapply STTyProj1.
+    apply STTyVar.
+    apply Ok_push; auto.
+    left; reflexivity.
+  - pose (topsig_dec t0).
+    inversion s; clear s.
+    assert (Ha : exists r, and_coercion t0 ((fun A : Type => STApp A (c A) (STProj2 A (STBVar A 0)))) = inl r /\ has_type_st Gamma (r var) (|t0|)) by (apply and_coercion_inl_typing; auto).
+    destruct Ha as [r [HCoerce HHasTy]].
+    rewrite HCoerce.
+    apply_fresh STTyLam' as x.
+    simpl.
+    unfold open; rewrite <- open_rec_term.
+    rewrite <- app_nil_l with (l := (extend x (STTuple (| t1 |) (| t2 |)) Gamma)).
+    apply typing_weaken; rewrite app_nil_l.
+    apply HHasTy.
+    apply Ok_push; auto.
+    now apply typing_gives_terms in HHasTy.
+    eapply and_coercion_inr in H2.
+    rewrite H2; simpl.
+    apply_fresh STTyLam' as x; cbn.
+    eapply STTyApp.
+    rewrite <- open_rec_term.
+    apply typing_weaken_extend.
+    apply IHsub.
+    assumption.
+    now apply typing_gives_terms in IHsub.
+    eapply STTyProj2.
+    apply STTyVar.
+    apply Ok_push; auto.
+    left; reflexivity.
+  - apply_fresh STTyLam' as x; cbn; apply STTyUnit.
+    apply Ok_push; auto.
+Qed.  
+  
+Lemma and_coercion_proj1_term :
+  forall t0 (c : Exp),
+    STTerm (c var) ->
+    STTerm (STLam' var (join_sum (and_coercion t0 (fun A : Type => (STApp A (c A) (STProj1 A (STBVar A 0)))))
+        var)).
+Proof.
+  intros.
+  apply_fresh STTerm_Lam' as x; unfold open; simpl.
+  pose (topsig_dec t0).
+  inversion s; clear s.
+  assert (exists r : Exp, and_coercion t0 (fun A : Type =>
+                          STApp A (c A) (STProj1 A (STBVar A 0))) = inl r /\ STTerm (r var)).
+  apply and_coercion_inl_term; auto.
+  inversion H1.
+  inversion H2.
+  rewrite H3.
+  simpl.
+  rewrite <- open_rec_term; auto.
+  eapply and_coercion_inr in H0.
+  rewrite H0.
+  simpl.
+  apply STTerm_App; auto.
+  rewrite <- open_rec_term; auto.
 Qed.
 
 Lemma and_coercion_proj2_term :
-  forall t0 n (c : Exp),
+  forall t0 (c : Exp),
     STTerm (c var) ->
-    STTerm (and_coercion t0 (fun A : Type =>
-                               STLam' A (STApp A (c A) (STProj2 A
-                                                                (STBVar A 0)))) n
-        var).
+    STTerm (STLam' var (join_sum (and_coercion t0 (fun A : Type => (STApp A (c A) (STProj2 A (STBVar A 0)))))
+        var)).
 Proof.
   intros.
-  generalize dependent n.
-  induction t0; intros; simpl; try apply IHt0_2.
-  - apply_fresh STTerm_Lam' as x; cbn.
-    apply STTerm_App; auto.
-    rewrite <- open_rec_term; auto.
-  - apply_fresh STTerm_Lam' as x; cbn.
-    apply STTerm_App; auto.
-    rewrite <- open_rec_term; auto.
-  - induction n.
-    simpl.
-    apply_fresh STTerm_Lam' as x; auto.
-    simpl.
-    apply_fresh STTerm_Lam' as x; simpl in *.
-    unfold open.
-    rewrite <- open_rec_term; auto.
+  apply_fresh STTerm_Lam' as x; unfold open; simpl.
+  pose (topsig_dec t0).
+  inversion s; clear s.
+  assert (exists r : Exp, and_coercion t0 (fun A : Type =>
+                          STApp A (c A) (STProj2 A (STBVar A 0))) = inl r /\ STTerm (r var)).
+  apply and_coercion_inl_term; auto.
+  inversion H1.
+  inversion H2.
+  rewrite H3.
+  simpl.
+  rewrite <- open_rec_term; auto.
+  eapply and_coercion_inr in H0.
+  rewrite H0.
+  simpl.
+  apply STTerm_App; auto.
+  rewrite <- open_rec_term; auto.
 Qed.
 
-  
 Lemma coercions_produce_terms :
   forall E A B, sub A B E -> STTerm (E var).
 Proof.
@@ -2110,741 +2343,6 @@ Proof.
   - apply_fresh STTerm_Lam' as x; cbn.
     apply STTerm_Unit.
 Qed.
-
-Hint Resolve coercions_produce_terms.
-
-Inductive TopSig : PTyp -> Prop :=
-  | TopSigF : forall A B, TopSig B -> TopSig (Fun A B)
-  | TopSigT : TopSig TopT.                    
-
-Print genCoerce.
-Print and_coercion.
-
-Fixpoint and_type (p : PTyp) (seed : PTyp) {struct p} : STyp :=
-  match p with
-  | PInt    => STUnitT
-  | Fun A B => STFun (|seed|) (and_type B A)
-  | And A B => STUnitT
-  | TopT    => STFun (|seed|) STUnitT
-  end.
-
-Lemma and_type_has_type_st :
-  forall t e r Gamma,
-    TopSig t ->
-    and_coercion t e 0 = r ->
-    exists A, has_type_st Gamma (STLam' _ (r var)) (and_type t A).
-Proof.
-  intros.
-  induction H.
-  
-Admitted.
-
-Fixpoint genCoerce' (n : nat) : Exp :=
-  match n with
-    | 0 => fun A : Type => STUnit A
-    | S m => fun A : Type => STLam' A (genCoerce' m A)
-  end.
-
-Fixpoint and_coercion' (t : PTyp) (e : Exp) (n : nat) {struct t} : Exp :=
-  match t with
-    | PInt    => e
-    | Fun _ B => and_coercion' B e (S n)
-    | And _ _ => e
-    | TopT    => genCoerce' n
-  end.
-
-Print genCoerce.
-
-Fixpoint and_coercion2 (t : PTyp) (e : Exp) {struct t} : sum Exp Exp :=
-  match t with
-    | PInt    => inr e
-    | Fun _ B => match (and_coercion2 B e) with
-                  | inl l => inl (fun A : Type => STLam' A (l A))
-                  | inr r => inr r
-                 end 
-    | And _ _ => inr e
-    | TopT    => inl (fun A : Type =>  STLam' A (STUnit A))
-  end.
-
-Lemma and_type_has_type_st' :
-  forall t e,
-    TopSig t ->
-    exists r, and_coercion2 t e = inl r.  
-Proof.
-  intros.
-  induction H.
-  destruct IHTopSig.
-  exists (fun A : Type => STLam' A (x A)).
-  simpl.
-  rewrite H0.
-  reflexivity.
-  exists (fun A : Type =>  STLam' A (STUnit A)).
-  now simpl.
-Qed.
-  
-(*
-Inductive and_coercion_def : PTyp -> Exp -> Exp -> Prop :=
-  | CPInt : forall e1, and_coercion_def PInt e1 e1
-  | CTopT : forall e1, and_coercion_def TopT e1 (fun T => STLam' T (STUnit _))
-  | CFun1 : forall A B e1 e2,
-              TopSig B ->
-              and_coercion_def B e1 e2 ->
-              and_coercion_def (Fun A B) e1 (fun T => STLam' T (e2 T))
-  | CFun2 : forall A B e1,
-              not (TopSig B) ->
-              and_coercion_def B e1 e1 ->
-              and_coercion_def (Fun A B) e1 e1
-  | CAnd : forall e1 A B, and_coercion_def (And A B) e1 e1.
-
-Check and_coercion_def_ind.
-
-Definition and_coercion_top_sig_ind :
-  forall (P : PTyp -> Exp -> Exp -> Prop),
-       (forall e1 : Exp, P TopT e1 (fun T : Type => STLam' T (STUnit T))) ->
-       (forall (A B : PTyp) (e1 e2 : Exp),
-        TopSig (Fun A B) ->
-        and_coercion_def B e1 e2 ->
-        P B e1 e2 -> P (Fun A B) e1 (fun T : Type => STLam' T (e2 T))) ->
-    forall t e r, and_coercion_def t e r -> TopSig t -> P t e r.
-  intros.
-  induction H1.
-  inversion H2.
-  auto.
-  apply H0; auto.
-  inversion H2; contradiction.
-  inversion H2.
-Defined.  
-*)
-
-Lemma and_coercion_rewrite_topsig :
-  forall t e r n,
-    TopSig t ->
-    and_coercion t e n var = r ->
-    exists m, genCoerce m var = r.              
-Proof.
-  intros.
-  generalize dependent n.
-  induction H; intros.
-  simpl in H0.
-  now apply IHTopSig in H0.
-  simpl in *.
-  now exists n.
-Qed.
-
-(*
-Inductive CountLam : PTyp -> nat -> Prop :=
-  | ZLam : CountLam TopT 0 
-  | SLam : forall t A n, CountLam t n ->
-                    CountLam (Fun A t) (S n).
-
-Lemma test :
-  forall B n e r,
-    TopSig B ->
-    and_coercion B e (S n) var = STLam' var r ->
-    and_coercion B e n var = r.
-Proof.
-Admitted.
-  
-Lemma and_coercion_rewrite_topsig' :
-  forall t e (r : SExp var) n,
-    TopSig t ->
-    and_coercion t e n var = r ->
-    exists m, genCoerce m var = r /\ CountLam t m.              
-Proof.
-  intros.
-  generalize dependent n.
-  generalize dependent r.
-  generalize dependent e.
-  dependent induction H; intros.
-  induction r; try now (
-  simpl in H0;
-  apply IHTopSig in H0;
-  inversion H0; inversion H1;
-  unfold genCoerce in H2;
-  destruct x; inversion H2).
-
-  simpl in H0.
-  apply test in H0.
-  apply IHTopSig in H0.
-  inversion H0.
-  exists (S x).
-  inversion H1.
-  split.
-  simpl.
-  apply f_equal; auto.
-  apply SLam; auto.
-  auto.
-
-  simpl in H0.
-  
-Admitted.
-*)
-Lemma and_coercion_rewrite_not_topsig : 
-  forall t e r n,
-    not (TopSig t) ->
-    and_coercion t e n = r ->
-    e = r.
-Proof.
-  intros.
-  generalize dependent n.
-  induction t0; intros.
-  now simpl in H0.
-  eapply IHt0_2.
-  unfold not; intros; apply H.
-  apply TopSigF.
-  assumption.
-  simpl in H0.
-  apply H0.
-  now simpl in H0.
-  exfalso; apply H; apply TopSigT.
-Qed.  
-
-Lemma topsig_dec : forall t, sumbool (TopSig t) (not (TopSig t)).
-Proof.
-  intro t.
-  induction t.
-  - right; unfold not; intros HInv; inversion HInv. 
-  - inversion IHt2.
-    left.
-    apply TopSigF.
-    apply H.
-    right.
-    unfold not; intros HInv; inversion HInv; subst.
-    contradiction.
-  - right; unfold not; intros HInv; inversion HInv.
-  - left; apply TopSigT.
-Qed.    
-    
-Lemma and_coercion_rewrite' :
-  forall t e (r : SExp var) n, and_coercion t e n var = r ->
-                          (r = (e var) \/ exists m, r = genCoerce m var).
-Proof.
-  intros.
-  generalize dependent n.
-  induction t0; intros.
-  simpl; auto.
-  simpl in H.
-  eapply IHt0_2.
-  apply H.
-  simpl; auto.
-  unfold and_coercion in H.
-  right; exists n; auto.
-Qed.
-
-Fixpoint and_coercion3 (t : PTyp) (e : Exp) {struct t} : sum Exp Exp :=
-  match t with
-    | PInt    => inr e
-    | Fun _ B => match (and_coercion3 B e) with
-                  | inl l => inl (fun A : Type => STLam' A (l A))
-                  | inr r => inr r
-                 end 
-    | And _ _ => inr e
-    | TopT    => inl (fun A => (STUnit A))
-  end.
-
-Definition join_sum : forall {A}, A + A -> A.
-  intros A H; destruct H as [a | a]; exact a.
-Defined.
-
-Inductive sub' : PTyp -> PTyp -> Exp -> Prop :=
-  | SSInt : sub' PInt PInt (fun A => STLam' _ (STBVar _ 0))
-  | SSFun : forall o1 o2 o3 o4 c1 c2, sub' o3 o1 c1 -> sub' o2 o4 c2 -> 
-     sub' (Fun o1 o2) (Fun  o3 o4) (fun A => STLam' _ ( 
-       STLam' _ (STApp _ (c2 A) (STApp _ (STBVar _ 1) (STApp _ (c1 A) (STBVar _ 0))))))
-  | SSAnd1 : forall t t1 t2 c1 c2, sub' t t1 c1 -> sub' t t2 c2 -> 
-     sub' t (And  t1 t2) (fun A => STLam' _ (
-       STPair _ (STApp _ (c1 A) (STBVar _ 0)) (STApp _ (c2 A) (STBVar _ 0))))
-  | SSAnd2 : forall t t1 t2 c, sub' t1 t c -> Atomic t ->
-     sub' (And  t1 t2) t (fun A => STLam' _ (join_sum (and_coercion3 t (fun A => (
-       (STApp _ (c A) (STProj1 _ (STBVar _ 0)))))) A))
-  | SSAnd3 : forall t t1 t2 c, sub' t2 t c -> Atomic t ->
-     sub' (And  t1 t2) t (fun A => STLam' _ (join_sum (and_coercion3 t (fun A => (
-       (STApp _ (c A) (STProj2 _ (STBVar _ 0)))))) A))
-  | SSTop : forall t, sub' t TopT (fun A => STLam' _ (STUnit _)).
-
-Lemma and_type_term3 :
-  forall {t e},
-    TopSig t ->
-    exists r, and_coercion3 t e = inl r /\ STTerm (r var).  
-Proof.
-  intros.
-  induction H.
-  inversion IHTopSig.
-  exists (fun A : Type => STLam' A (x A)).
-  inversion H0.
-  split.
-  simpl.
-  rewrite H1.
-  reflexivity.
-  apply_fresh STTerm_Lam' as x.
-  unfold open; rewrite <- open_rec_term; auto.
-  exists (fun A : Type => STUnit A); auto.
-Qed.
-  
-Lemma and_type_has_type_st3 :
-  forall {t e Gamma},
-    ok Gamma ->
-    TopSig t ->
-    exists r, and_coercion3 t e = inl r /\ has_type_st Gamma (r var) (|t|).  
-Proof.
-  intros.
-  induction H0.
-  destruct IHTopSig.
-  exists (fun A : Type => STLam' A (x A)).
-  simpl.
-  destruct H1.
-  rewrite H1.
-  split.
-  reflexivity.
-  apply_fresh STTyLam' as v.
-  unfold open.
-  rewrite <- open_rec_term.
-  rewrite <- app_nil_l with (l := extend v (| A |) Gamma).
-  apply typing_weaken; rewrite app_nil_l.
-  apply H2.
-  apply Ok_push; assumption.
-  now apply typing_gives_terms in H2.
-  exists (fun A : Type =>  STUnit A).
-  split.
-  now simpl.
-  simpl.
-  apply STTyUnit.
-  auto.
-Qed.
-
-Lemma and_type_has_type_st3_not_topsig :
-  forall {t e},
-    not (TopSig t) ->
-    and_coercion3 t e = inr e.
-Proof.
-  intros.
-  generalize dependent e.
-  induction t0; try simpl; auto.
-  intros.
-  assert (not (TopSig t0_2)).
-  unfold not; intros HTS; apply H.
-  apply TopSigF; apply HTS.
-  apply IHt0_2 with (e := e) in H0.
-  rewrite H0.
-  reflexivity.
-  exfalso; apply H; apply TopSigT.
-Qed.
-  
-Lemma type_correct_coercions' :
-  forall Gamma A B E, sub' A B E ->
-             ok Gamma -> 
-             has_type_st Gamma (E var) (STFun (|A|) (|B|)) .
-Proof.
-  intros.
-  induction H.
-  (* Case SInt *)
-  - simpl.
-    apply_fresh STTyLam' as x; cbn.
-    simpl; apply STTyVar.
-    apply Ok_push; auto.
-    left; simpl; auto.
-  (* Case SFun *)
-  - apply_fresh STTyLam' as x; cbn.
-    apply_fresh STTyLam' as y; cbn.
-    apply STTyApp with (A := (| o2 |)).
-    rewrite <- open_rec_term.
-    rewrite <- open_rec_term.
-    repeat apply typing_weaken_extend.
-    assumption.
-    assumption. 
-    simpl.
-    not_in_L y.
-    apply MSetProperties.Dec.F.add_iff in H4; inversion H4.
-    exfalso; apply H2; apply MSetProperties.Dec.F.singleton_2; auto.
-    assumption.
-    now apply typing_gives_terms in IHsub'2.
-    rewrite <- open_rec_term.
-    now apply typing_gives_terms in IHsub'2.
-    now apply typing_gives_terms in IHsub'2.
-    eapply STTyApp.
-    apply STTyVar.
-    apply Ok_push.
-    apply Ok_push.
-    assumption.
-    assumption.
-    not_in_L y.
-    not_in_L x.
-    right; left; reflexivity.
-    apply STTyApp with (A := (| o3 |)).
-    rewrite <- open_rec_term.
-    rewrite <- open_rec_term.
-    repeat apply typing_weaken_extend.
-    assumption.
-    assumption. 
-    simpl.
-    not_in_L y.
-    apply MSetProperties.Dec.F.add_iff in H4; inversion H4.
-    exfalso; apply H2; apply MSetProperties.Dec.F.singleton_2; auto.
-    assumption.
-    now apply typing_gives_terms in IHsub'1.
-    rewrite <- open_rec_term; now apply typing_gives_terms in IHsub'1.
-    apply STTyVar.
-    apply Ok_push.
-    apply Ok_push.
-    assumption.
-    assumption.
-    simpl.
-    rewrite union_spec in Fry.
-    apply not_or_and in Fry.
-    inversion Fry.
-    unfold not; intros.
-    apply MSetProperties.Dec.F.add_iff in H4.
-    inversion H4.
-    apply H2.
-    apply MSetProperties.Dec.F.singleton_2; assumption.
-    contradiction.
-    left; reflexivity.
-  (* Case SAnd1 *)
-  - apply_fresh STTyLam' as x; cbn.
-    apply STTyPair.
-    eapply STTyApp.
-    rewrite <- open_rec_term.
-    apply typing_weaken_extend.
-    apply IHsub'1.
-    assumption.
-    now apply typing_gives_terms in IHsub'1.
-    apply STTyVar.
-    apply Ok_push; auto.
-    left; reflexivity.
-    eapply STTyApp.
-    rewrite <- open_rec_term.
-    apply typing_weaken_extend.
-    apply IHsub'2.
-    assumption.
-    now apply typing_gives_terms in IHsub'2.
-    apply STTyVar.
-    apply Ok_push; auto.
-    left; reflexivity.
-  - pose (topsig_dec t0).
-    inversion s; clear s.
-    assert (Ha : exists r, and_coercion3 t0 ((fun A : Type => STApp A (c A) (STProj1 A (STBVar A 0)))) = inl r /\ has_type_st Gamma (r var) (|t0|)) by (apply and_type_has_type_st3; auto).
-    destruct Ha as [r [HCoerce HHasTy]].
-    rewrite HCoerce.
-    apply_fresh STTyLam' as x.
-    simpl.
-    unfold open; rewrite <- open_rec_term.
-    rewrite <- app_nil_l with (l := (extend x (STTuple (| t1 |) (| t2 |)) Gamma)).
-    apply typing_weaken; rewrite app_nil_l.
-    apply HHasTy.
-    apply Ok_push; auto.
-    now apply typing_gives_terms in HHasTy.
-    eapply and_type_has_type_st3_not_topsig in H2.
-    rewrite H2; simpl.
-    apply_fresh STTyLam' as x; cbn.
-    eapply STTyApp.
-    rewrite <- open_rec_term.
-    apply typing_weaken_extend.
-    apply IHsub'.
-    assumption.
-    now apply typing_gives_terms in IHsub'.
-    eapply STTyProj1.
-    apply STTyVar.
-    apply Ok_push; auto.
-    left; reflexivity.
-  - pose (topsig_dec t0).
-    inversion s; clear s.
-    assert (Ha : exists r, and_coercion3 t0 ((fun A : Type => STApp A (c A) (STProj2 A (STBVar A 0)))) = inl r /\ has_type_st Gamma (r var) (|t0|)) by (apply and_type_has_type_st3; auto).
-    destruct Ha as [r [HCoerce HHasTy]].
-    rewrite HCoerce.
-    apply_fresh STTyLam' as x.
-    simpl.
-    unfold open; rewrite <- open_rec_term.
-    rewrite <- app_nil_l with (l := (extend x (STTuple (| t1 |) (| t2 |)) Gamma)).
-    apply typing_weaken; rewrite app_nil_l.
-    apply HHasTy.
-    apply Ok_push; auto.
-    now apply typing_gives_terms in HHasTy.
-    eapply and_type_has_type_st3_not_topsig in H2.
-    rewrite H2; simpl.
-    apply_fresh STTyLam' as x; cbn.
-    eapply STTyApp.
-    rewrite <- open_rec_term.
-    apply typing_weaken_extend.
-    apply IHsub'.
-    assumption.
-    now apply typing_gives_terms in IHsub'.
-    eapply STTyProj2.
-    apply STTyVar.
-    apply Ok_push; auto.
-    left; reflexivity.
-  - apply_fresh STTyLam' as x; cbn; apply STTyUnit.
-    apply Ok_push; auto.
-Qed.  
-  
-Lemma and_coercion_proj1_term' :
-  forall t0 (c : Exp),
-    STTerm (c var) ->
-    STTerm (STLam' var (join_sum (and_coercion3 t0 (fun A : Type => (STApp A (c A) (STProj1 A (STBVar A 0)))))
-        var)).
-Proof.
-  intros.
-  apply_fresh STTerm_Lam' as x; unfold open; simpl.
-  pose (topsig_dec t0).
-  inversion s; clear s.
-  assert (exists r : Exp, and_coercion3 t0 (fun A : Type =>
-                          STApp A (c A) (STProj1 A (STBVar A 0))) = inl r /\ STTerm (r var)).
-  apply and_type_term3; auto.
-  inversion H1.
-  inversion H2.
-  rewrite H3.
-  simpl.
-  rewrite <- open_rec_term; auto.
-  eapply and_type_has_type_st3_not_topsig in H0.
-  rewrite H0.
-  simpl.
-  apply STTerm_App; auto.
-  rewrite <- open_rec_term; auto.
-Qed.
-
-Lemma and_coercion_proj2_term' :
-  forall t0 (c : Exp),
-    STTerm (c var) ->
-    STTerm (STLam' var (join_sum (and_coercion3 t0 (fun A : Type => (STApp A (c A) (STProj2 A (STBVar A 0)))))
-        var)).
-Proof.
-  intros.
-  apply_fresh STTerm_Lam' as x; unfold open; simpl.
-  pose (topsig_dec t0).
-  inversion s; clear s.
-  assert (exists r : Exp, and_coercion3 t0 (fun A : Type =>
-                          STApp A (c A) (STProj2 A (STBVar A 0))) = inl r /\ STTerm (r var)).
-  apply and_type_term3; auto.
-  inversion H1.
-  inversion H2.
-  rewrite H3.
-  simpl.
-  rewrite <- open_rec_term; auto.
-  eapply and_type_has_type_st3_not_topsig in H0.
-  rewrite H0.
-  simpl.
-  apply STTerm_App; auto.
-  rewrite <- open_rec_term; auto.
-Qed.
-
-Lemma coercions_produce_terms' :
-  forall E A B, sub' A B E -> STTerm (E var).
-Proof.
-  intros.
-  induction H.
-  (* Case SInt *)
-  - apply_fresh STTerm_Lam' as x. cbn; auto.
-  (* Case SFun *)
-  - apply_fresh STTerm_Lam' as x; cbn.
-    apply_fresh STTerm_Lam' as y; cbn.
-    apply STTerm_App.
-    repeat rewrite <- open_rec_term; assumption.
-    apply STTerm_App.
-    apply STTerm_Var.
-    apply STTerm_App; [ repeat rewrite <- open_rec_term; auto | apply STTerm_Var ].
-  (* Case SAnd1 *)
-  - apply_fresh STTerm_Lam' as x; cbn.
-    apply STTerm_Pair.
-    apply STTerm_App; repeat rewrite <- open_rec_term; auto.
-    rewrite <- open_rec_term; auto.
-  (* Case SAnd2 *)
-  - apply and_coercion_proj1_term'; auto.
-  (* Case SAnd3 *)
-  - apply and_coercion_proj2_term'; auto.
-  (* Case STop *)
-  - apply_fresh STTerm_Lam' as x; cbn.
-    apply STTerm_Unit.
-Qed.
-
-(* Subtyping rules produce type-correct coercions: Lemma 3 *)
-Lemma type_correct_coercions' :
-  forall Gamma A B E, sub A B E ->
-             ok Gamma -> 
-             has_type_st Gamma (E var) (STFun (|A|) (|B|)) .
-Proof.
-  intros.
-  pose (topsig_dec B).
-  inversion s; clear s.
-  induction H.
-  admit.
-  admit.
-  admit.
-  remember (and_coercion t0
-        (fun A : Type => STLam' A (STApp A (c A) (STProj1 A (STBVar A 0)))) 0
-        var).
-  symmetry in Heqs.
-  apply (and_coercion_rewrite_topsig _ _ _ _ H1) in Heqs.
-
-  (*
-  inversion Heqs.
-  induction x.
-  rewrite <- H3.
-  simpl.
-  *)
-  
-  (* eapply (and_coercion_rewrite_topsig _ _ _ _ H1) in Heqs. *)
-Admitted.
-  
-(* Subtyping rules produce type-correct coercions: Lemma 3 *)
-Lemma type_correct_coercions :
-  forall Gamma A B E, sub A B E ->
-             ok Gamma -> 
-             has_type_st Gamma (E var) (STFun (|A|) (|B|)) .
-Proof.
-  intros.
-  induction H. Print sub.
-  (* Case SInt *)
-  - simpl.
-    apply_fresh STTyLam' as x; cbn.
-    simpl; apply STTyVar.
-    apply Ok_push; auto.
-    left; simpl; auto.
-  (* Case SFun *)
-  - apply_fresh STTyLam' as x; cbn.
-    apply_fresh STTyLam' as y; cbn.
-    apply STTyApp with (A := (| o2 |)).
-    rewrite <- open_rec_term.
-    rewrite <- open_rec_term.
-    repeat apply typing_weaken_extend.
-    assumption.
-    assumption. 
-    simpl.
-    not_in_L y.
-    apply MSetProperties.Dec.F.add_iff in H4; inversion H4.
-    exfalso; apply H2; apply MSetProperties.Dec.F.singleton_2; auto.
-    assumption.
-    eapply coercions_produce_terms; apply H1.
-    rewrite <- open_rec_term; eapply coercions_produce_terms; apply H1.
-    eapply STTyApp.
-    apply STTyVar.
-    apply Ok_push.
-    apply Ok_push.
-    assumption.
-    assumption.
-    not_in_L y.
-    not_in_L x.
-    right; left; reflexivity.
-    apply STTyApp with (A := (| o3 |)).
-    rewrite <- open_rec_term.
-    rewrite <- open_rec_term.
-    repeat apply typing_weaken_extend.
-    assumption.
-    assumption. 
-    simpl.
-    not_in_L y.
-    apply MSetProperties.Dec.F.add_iff in H4; inversion H4.
-    exfalso; apply H2; apply MSetProperties.Dec.F.singleton_2; auto.
-    assumption.
-    eapply coercions_produce_terms; apply H.
-    rewrite <- open_rec_term; now apply coercions_produce_terms in H.
-    apply STTyVar.
-    apply Ok_push.
-    apply Ok_push.
-    assumption.
-    assumption.
-    simpl.
-    rewrite union_spec in Fry.
-    apply not_or_and in Fry.
-    inversion Fry.
-    unfold not; intros.
-    apply MSetProperties.Dec.F.add_iff in H4.
-    inversion H4.
-    apply H2.
-    apply MSetProperties.Dec.F.singleton_2; assumption.
-    contradiction.
-    left; reflexivity.
-  (* Case SAnd1 *)
-  - apply_fresh STTyLam' as x; cbn.
-    apply STTyPair.
-    eapply STTyApp.
-    rewrite <- open_rec_term.
-    apply typing_weaken_extend.
-    apply IHsub1.
-    assumption.
-    now apply coercions_produce_terms in H.
-    apply STTyVar.
-    apply Ok_push; auto.
-    left; reflexivity.
-    eapply STTyApp.
-    rewrite <- open_rec_term.
-    apply typing_weaken_extend.
-    apply IHsub2.
-    assumption.
-    now apply coercions_produce_terms in H1.
-    apply STTyVar.
-    apply Ok_push; auto.
-    left; reflexivity.
-  (* Case SAnd2 *)
-  - generalize dependent IHsub.
-    induction t0; intros.
-    simpl.
-    apply_fresh STTyLam' as x; cbn.
-    eapply STTyApp.
-    rewrite <- open_rec_term.
-    apply typing_weaken_extend.
-    subst; apply IHsub.
-    assumption.
-    now apply coercions_produce_terms in H.
-    eapply STTyProj1.
-    apply STTyVar.
-    apply Ok_push; auto.
-    left; reflexivity.
-    induction t0_2.
-    simpl; apply_fresh STTyLam' as x; cbn.
-    eapply STTyApp.
-    rewrite <- open_rec_term.
-    apply typing_weaken_extend.
-    subst; apply IHsub.
-    assumption.
-    now apply coercions_produce_terms in H.
-    eapply STTyProj1.
-    apply STTyVar.
-    apply Ok_push; auto.
-    left; reflexivity.
-    simpl in *.
-    destruct t
-    SearchAbout Atomic.
-    admit.
-
-    Print sub. inversion H. simpl.
-    
-    induction H1.
-    apply_fresh STTyLam' as x; cbn.
-    eapply STTyApp.
-    rewrite <- open_rec_term.
-    apply typing_weaken_extend.
-    subst; apply IHsub.
-    assumption.
-    now apply coercions_produce_terms in H.
-    eapply STTyProj1.
-    apply STTyVar.
-    apply Ok_push; auto.
-    left; reflexivity. simpl.
-    admit. (* admit.
-    simpl. apply_fresh STTyLam' as x; simpl in *.
-    unfold open.
-    rewrite <- open_rec_term.
-    apply STTyUnit.
-    apply Ok_push; auto.
-    auto. *)
-  (* SAnd3 *)
-  - inversion H1.
-    apply_fresh STTyLam' as x; cbn.
-    eapply STTyApp.
-    rewrite <- open_rec_term.
-    apply typing_weaken_extend.
-    subst; apply IHsub.
-    assumption.
-    now apply coercions_produce_terms in H.
-    eapply STTyProj2.
-    apply STTyVar.
-    apply Ok_push; auto.
-    left; reflexivity.
-    admit.
-  (* STop *)
-  - apply_fresh STTyLam' as x; cbn. apply STTyUnit.
-    apply Ok_push; auto.
-Admitted.
-
   
 (* Type preservation: Theorem 1 *)
 Lemma type_preservation :
@@ -2891,8 +2389,6 @@ Proof.
 Defined.
     
 (* Completeness *)
-
-(* An auxiliary lemma that, given suitable pre-conditions, I think it will hold. *)
 
 Lemma erasure_open : forall t1 n t0 x,
   not (In x (fv_source t0)) ->
